Lp2lc/Active/DTLC/Impl.lean
@@ -10,9 +10,10 @@ inductive Symbol where -- no constructor, it can only be retrieved from FBound
 
 namespace Symbolic
 
-abbrev Typ (ByteCode : Type) := AST.Typ Symbol ByteCode
-abbrev Val (ByteCode : Type) := AST.Val Symbol ByteCode
-abbrev Trm (ByteCode : Type) := AST.Trm Symbol ByteCode
+abbrev ByteCode := String
+abbrev Typ := AST.Typ Symbol ByteCode
+abbrev Val := AST.Val Symbol ByteCode
+abbrev Trm := AST.Trm Symbol ByteCode
 
 end Symbolic
 
